A test that drives the record layer.
At least the first test cases gives the desired output. I had to fill out some
dummy definitions, though.

src/tls/TLSConstants.fst
@@ -68,7 +68,8 @@ assume val strongAuthAlg: ProtocolVersion -> aeAlg -> Tot bool
 //  | MtE _ m | MACOnly m   -> int_cma (macAlg_of_id i)
 //  | AEAD e m -> strongAEADalg
 
-assume val strongAEAlg: ProtocolVersion -> aeAlg -> Tot bool
+val strongAEAlg: ProtocolVersion -> aeAlg -> Tot bool
+let strongAEAlg _ _ = false
 // let strongAEAlg pv ae = match ae with
 //    | AEAD e m -> true
 //    | MtE _ -> false
